ambient_capabilities_coq_model/assert.v
@@ -4,6 +4,7 @@ Require Import List.
 Require Import CpdtTactics.
 Require Import common.
 Require Import language_def.
+Require Import subst.
 Require Export operational_semantics.
 
 Require Export Coq.Numbers.BinNums.
@@ -12,7 +13,12 @@ Require Export ZArith.
 Module Assert.
 
   Import LanguageDefinition.
+  Import SubstDefn.
   Import OperationalSemantics.
+
+
+  Declare Scope assert_scope.
+
 
   Fixpoint interpret_αp (p : path)(σ : config)(α : addr) : option val :=
     match p with
@@ -64,50 +70,6 @@ Module Assert.
   Definition protected_from (M : module)(σ : config)(α_orig α : addr) :=
     forall p, interpret_αp p σ α_orig = Some (v_addr α) -> is_protected_path M σ α_orig p.
 
-  Class Subst (A B C : Type) : Type :=
-    {
-      sbst : A -> B -> C -> A
-    }.
-
-  Notation "'[' c '/s' b ']' a" := (sbst a b c)(at level 80).
-
-  #[global] Instance exp_subst : Subst exp nat addr:=
-    {
-      sbst :=
-        fix sbst' e n α :=
-          match e with
-          | e_hole m  => if beq_nat n m
-                        then e_val (v_addr α)
-                        else e_hole m
-          | e_fld e' f => e_fld (sbst' e' n α) f
-          | e_class e' C => e_class (sbst' e' n α) C
-          | e_ghost e0 g e1 => e_ghost (sbst' e0 n α) g (sbst' e1 n α)
-          | e_if e0 e1 e2 => e_if (sbst' e0 n α) (sbst' e1 n α) (sbst' e2 n α)
-          | _ => e
-          end
-    }.
-
-  #[global] Instance asrtSubst : Subst asrt nat addr:=
-    {
-      sbst :=
-        fix sbst' A n α :=
-          match A with
-          | a_exp e     => a_exp ([ α /s n ] e)
-          | A1 ∧ A2     => (sbst' A1 n α) ∧ (sbst' A2 n α)
-          | A1 ∨ A2     => (sbst' A1 n α) ∨ (sbst' A2 n α)
-          | ¬ A         => ¬ (sbst' A n α)
-          (*)        | A1 ⟶ A2   => (sbst' A1 n α) ⟶ (sbst' A2 n α)*)
-
-          | a_all C A  => a_all C (sbst' A (S n) α)
-          | a_ex C A   => a_ex C (sbst' A (S n) α)
-
-          | a_intl e => a_intl ([α /s n] e)
-          | a_extl e => a_extl ([α /s n] e)
-
-          | a_prt_frm e1 e2 => a_prt_frm ([α /s n] e1) ([α /s n] e2)
-          | a_prt e => a_prt ([α /s n] e)
-          end
-    }.
 
   Inductive sat : module -> config -> asrt -> Prop :=
   | sat_exp : forall M σ e, eval M σ e v_true ->
@@ -253,5 +215,9 @@ M ⊢ {P1 /\ P2} s {Q1 /\ Q2}!!!!!!!!!!!!!!!!!!!!!!!!!!!!!!!!!!!!
       with nsat_mut_ind := Induction for nsat Sort Prop.
 
   Combined Scheme sat_mutind from sat_mut_ind, nsat_mut_ind.
+
+  #[export] Hint Constructors sat : assert_db.
+
+  Close Scope assert_scope.
 
 End Assert.
